proofs

libcrux-ml-kem/src/vector/avx2.rs
@@ -237,8 +237,8 @@ impl Operations for SIMD256Vector {
 
     #[requires(fstar!("Spec.Utils.is_i16b 1664 zeta0 /\\ Spec.Utils.is_i16b 1664 zeta1 /\\
                        Spec.Utils.is_i16b 1664 zeta2 /\\ Spec.Utils.is_i16b 1664 zeta3 /\\
-                       Spec.Utils.is_i16b_array 3228 (impl.f_repr ${lhs}) /\\
-                       Spec.Utils.is_i16b_array 3228 (impl.f_repr ${rhs})"))]
+                       Spec.Utils.is_i16b_array 3328 (impl.f_repr ${lhs}) /\\
+                       Spec.Utils.is_i16b_array 3328 (impl.f_repr ${rhs})"))]
     #[ensures(|out| fstar!("Spec.Utils.is_i16b_array 3328 (impl.f_repr $out)"))]
     fn ntt_multiply(
         lhs: &Self,
