libcrux-ml-kem/src/vector/portable/ntt.rs
@@ -191,41 +191,35 @@ pub(crate) fn inv_ntt_layer_3_step(mut vec: PortableVector, zeta: i16) -> Portab
 /// The NIST FIPS 203 standard can be found at
 /// <https://csrc.nist.gov/pubs/fips/203/ipd>.
 #[inline(always)]
-#[hax_lib::fstar::options("--z3rlimit 200 --split_queries always --query_stats")]
-#[hax_lib::requires(fstar!("v i < 16 /\\ v j < 16 /\\ Spec.Utils.is_i16b 1664 $zeta /\\
-        Spec.Utils.is_i16b_array 3228 ${a}.f_elements /\\
-        Spec.Utils.is_i16b_array 3228 ${b}.f_elements "))]
+#[hax_lib::fstar::options("--z3rlimit 250 --split_queries always --query_stats --ext context_prune")]
+#[hax_lib::fstar::before(interface, "[@@ \"opaque_to_smt\"]")]
+#[hax_lib::requires(fstar!("v i < 8 /\\ Spec.Utils.is_i16b 1664 $zeta /\\
+        Spec.Utils.is_i16b_array 3328 ${a}.f_elements /\\
+        Spec.Utils.is_i16b_array 3328 ${b}.f_elements /\\
+        Spec.Utils.is_i16b_array 3328 ${out}.f_elements "))]
 #[hax_lib::ensures(|()| fstar!("
-        Spec.Utils.is_i16b_array 3328 ${out}.f_elements /\\
-        (forall k. (k <> v $i /\\ k <> v $j) ==> 
+        Spec.Utils.is_i16b_array 3328 ${out}_future.f_elements /\\
+        (forall k. (k < 2 * v $i \\/ k > 2 * v $i + 1) ==> 
                     Seq.index out_future.f_elements k == Seq.index out.f_elements k) /\\                 
-         (let ai = Seq.index ${a}.f_elements (v $i) in
-          let aj = Seq.index ${a}.f_elements (v $j) in
-          let bi = Seq.index ${b}.f_elements (v $i) in
-          let bj = Seq.index ${b}.f_elements (v $j) in
-          let oi = Seq.index out_future.f_elements (v $i) in
-          let oj = Seq.index out_future.f_elements (v $j) in
-          let (x,y) = 
-          Spec.MLKEM.Math.poly_base_case_multiply 
-             (v ai % 3329)
-             (v aj % 3329)
-             (v bi % 3329)
-             (v bj % 3329)
-             ((v zeta * 169) % 3329) in
-          ((x * 169) % 3329 == v oi % 3329) /\\
-           (y * 169) % 3329 == v oj % 3329)))"))]
+        (let ai = Seq.index ${a}.f_elements (2 * v $i) in
+         let aj = Seq.index ${a}.f_elements (2 * v $i + 1) in
+         let bi = Seq.index ${b}.f_elements (2 * v $i) in
+         let bj = Seq.index ${b}.f_elements (2 * v $i + 1) in
+         let oi = Seq.index out_future.f_elements (2 * v $i) in
+         let oj = Seq.index out_future.f_elements (2 * v $i + 1) in
+         ((v oi % 3329) == (((v ai * v bi + (v aj * v bj * v zeta * 169)) * 169) % 3329)) /\\
+         ((v oj % 3329) == (((v ai * v bj + v aj * v bi) * 169) % 3329)))"))]
 pub(crate) fn ntt_multiply_binomials(
     a: &PortableVector,
     b: &PortableVector,
     zeta: FieldElementTimesMontgomeryR,
     i: usize,
-    j: usize,
     out: &mut PortableVector,
 ) {
-    let ai = a.elements[i];
-    let bi = b.elements[i];
-    let aj = a.elements[j];
-    let bj = b.elements[j];
+    let ai = a.elements[2*i];
+    let bi = b.elements[2*i];
+    let aj = a.elements[2*i+1];
+    let bj = b.elements[2*i+1];
     hax_lib::fstar!("assert(Spec.Utils.is_i16b 3328 $ai);
                      assert(Spec.Utils.is_i16b 3328 $bi);
                      assert(Spec.Utils.is_i16b 3328 $aj);
@@ -250,6 +244,8 @@ pub(crate) fn ntt_multiply_binomials(
         (v $ai_bi_aj_bj * 169) % 3329;
         ( == ) { assert(v $ai_bi_aj_bj == v $ai_bi + v $aj_bj_zeta) }
         ((v $ai_bi + v $aj_bj_zeta) * 169) % 3329;
+        ( == ) { assert (v $ai_bi == v $ai * v $bi) }
+        (((v $ai * v $bi) + v $aj_bj_zeta) * 169) % 3329;
         ( == ) { assert (v $aj_bj_zeta == v $aj_bj * v $zeta) }
         (((v $ai * v $bi) + (v $aj_bj * v $zeta)) * 169) % 3329;
         ( == ) { Math.Lemmas.lemma_mod_mul_distr_l ((v ai * v bi) + (v aj_bj * v zeta)) 169 3329 }
@@ -277,8 +273,26 @@ pub(crate) fn ntt_multiply_binomials(
     hax_lib::fstar!("assert(Spec.Utils.is_i32b (3328*3328 + 3328*3328) ai_bj_aj_bi) ");
     hax_lib::fstar!("assert_norm (3328 * 3328 + 3328 * 3328 <= 3328 * pow2 15)");
     let o1 = montgomery_reduce_element(ai_bj_aj_bi);
-    out.elements[i] = o0;
-    out.elements[j] = o1;
+    hax_lib::fstar!("calc  ( == ) {
+        v $o1 % 3329;
+        ( == ) { () }
+        (v $ai_bj_aj_bi * 169) % 3329;
+        ( == ) { assert(v $ai_bj_aj_bi == v $ai_bj + v $aj_bi) }
+        ((v $ai_bj + v $aj_bi) * 169) % 3329;
+        ( == ) { assert (v ai_bj == v ai * v bj) }
+        ((v ai * v bj + v aj_bi) * 169) % 3329;
+        ( == ) { assert (v aj_bi == v aj * v bi) }
+        ((v ai * v bj + v aj * v bi) * 169) % 3329;
+    }");
+    let _out0 = out.elements;
+    out.elements[2*i] = o0;
+    out.elements[2*i+1] = o1;
+    hax_lib::fstar!("assert (Seq.index out.f_elements (2 * v i) == o0);
+                     assert (Seq.index out.f_elements (2 * v i + 1) == o1);
+                     assert (Spec.Utils.is_i16b_array 3328 out.f_elements);
+                     assert (forall k. (k <> 2 * v i /\\ k <> 2 * v i + 1) ==>
+                                        Seq.index out.f_elements k ==
+                                        Seq.index ${_out0} k)");
     hax_lib::fstar!("admit()");
 }
 
@@ -303,8 +317,8 @@ pub(crate) fn ntt_multiply_binomials(
         Spec.Utils.is_i16b 1664 $zeta1 /\\
         Spec.Utils.is_i16b 1664 $zeta2 /\\
         Spec.Utils.is_i16b 1664 $zeta3 /\\
-        Spec.Utils.is_i16b_array 3228 ${lhs}.f_elements /\\
-        Spec.Utils.is_i16b_array 3228 ${rhs}.f_elements "))]
+        Spec.Utils.is_i16b_array 3328 ${lhs}.f_elements /\\
+        Spec.Utils.is_i16b_array 3328 ${rhs}.f_elements "))]
 #[hax_lib::ensures(|result| fstar!("Spec.Utils.is_i16b_array 3328 ${result}.f_elements"))]
 pub(crate) fn ntt_multiply(
     lhs: &PortableVector,
@@ -323,14 +337,19 @@ pub(crate) fn ntt_multiply(
     hax_lib::fstar!("assert (Spec.Utils.is_i16b 1664 nzeta2)");
     hax_lib::fstar!("assert (Spec.Utils.is_i16b 1664 nzeta3)");
     let mut out = zero();
-    ntt_multiply_binomials(lhs, rhs, zeta0, 0, 1, &mut out);
-    ntt_multiply_binomials(lhs, rhs, nzeta0, 2, 3, &mut out);
-    ntt_multiply_binomials(lhs, rhs, zeta1, 4, 5, &mut out);
-    ntt_multiply_binomials(lhs, rhs, nzeta1, 6, 7, &mut out);
+    hax_lib::fstar!("assert (Spec.Utils.is_i16b_array 3328 out.f_elements)");
+    ntt_multiply_binomials(lhs, rhs, zeta0, 0, &mut out);
+    hax_lib::fstar!("assert (Spec.Utils.is_i16b_array 3328 out.f_elements)");
+    ntt_multiply_binomials(lhs, rhs, nzeta0, 1, &mut out);
+    hax_lib::fstar!("assert (Spec.Utils.is_i16b_array 3328 out.f_elements)");
+    ntt_multiply_binomials(lhs, rhs, zeta1, 2, &mut out);
+    hax_lib::fstar!("assert (Spec.Utils.is_i16b_array 3328 out.f_elements)");
+    ntt_multiply_binomials(lhs, rhs, nzeta1, 3, &mut out);
+    hax_lib::fstar!("assert (Spec.Utils.is_i16b_array 3328 out.f_elements)");
     hax_lib::fstar!("admit()");
-    ntt_multiply_binomials(lhs, rhs, zeta2, 8, 9, &mut out);
-    ntt_multiply_binomials(lhs, rhs, nzeta2, 10, 11, &mut out);
-    ntt_multiply_binomials(lhs, rhs, zeta3, 12, 13, &mut out);
-    ntt_multiply_binomials(lhs, rhs, nzeta3, 14, 15, &mut out);
+    ntt_multiply_binomials(lhs, rhs, zeta2, 4, &mut out);
+    ntt_multiply_binomials(lhs, rhs, nzeta2, 5, &mut out);
+    ntt_multiply_binomials(lhs, rhs, zeta3, 6, &mut out);
+    ntt_multiply_binomials(lhs, rhs, nzeta3, 7, &mut out);
     out
 }
