libcrux-ml-kem/proofs/fstar/extraction/Libcrux_ml_kem.Vector.Portable.Ntt.fst
@@ -173,18 +173,24 @@ let inv_ntt_layer_3_step
 
 #pop-options
 
-#push-options "--z3rlimit 200 --split_queries always --query_stats"
+#push-options "--z3rlimit 250 --split_queries always --query_stats --ext context_prune"
 
 let ntt_multiply_binomials
       (a b: Libcrux_ml_kem.Vector.Portable.Vector_type.t_PortableVector)
       (zeta: i16)
-      (i j: usize)
+      (i: usize)
       (out: Libcrux_ml_kem.Vector.Portable.Vector_type.t_PortableVector)
      =
-  let ai:i16 = a.Libcrux_ml_kem.Vector.Portable.Vector_type.f_elements.[ i ] in
-  let bi:i16 = b.Libcrux_ml_kem.Vector.Portable.Vector_type.f_elements.[ i ] in
-  let aj:i16 = a.Libcrux_ml_kem.Vector.Portable.Vector_type.f_elements.[ j ] in
-  let bj:i16 = b.Libcrux_ml_kem.Vector.Portable.Vector_type.f_elements.[ j ] in
+  let ai:i16 = a.Libcrux_ml_kem.Vector.Portable.Vector_type.f_elements.[ sz 2 *! i <: usize ] in
+  let bi:i16 = b.Libcrux_ml_kem.Vector.Portable.Vector_type.f_elements.[ sz 2 *! i <: usize ] in
+  let aj:i16 =
+    a.Libcrux_ml_kem.Vector.Portable.Vector_type.f_elements.[ (sz 2 *! i <: usize) +! sz 1 <: usize
+    ]
+  in
+  let bj:i16 =
+    b.Libcrux_ml_kem.Vector.Portable.Vector_type.f_elements.[ (sz 2 *! i <: usize) +! sz 1 <: usize
+    ]
+  in
   let _:Prims.unit =
     assert (Spec.Utils.is_i16b 3328 ai);
     assert (Spec.Utils.is_i16b 3328 bi);
@@ -211,6 +217,8 @@ let ntt_multiply_binomials
       (v ai_bi_aj_bj * 169) % 3329;
       ( == ) { assert (v ai_bi_aj_bj == v ai_bi + v aj_bj_zeta) }
       ((v ai_bi + v aj_bj_zeta) * 169) % 3329;
+      ( == ) { assert (v ai_bi == v ai * v bi) }
+      (((v ai * v bi) + v aj_bj_zeta) * 169) % 3329;
       ( == ) { assert (v aj_bj_zeta == v aj_bj * v zeta) }
       (((v ai * v bi) + (v aj_bj * v zeta)) * 169) % 3329;
       ( == ) { Math.Lemmas.lemma_mod_mul_distr_l ((v ai * v bi) + (v aj_bj * v zeta)) 169 3329 }
@@ -241,6 +249,20 @@ let ntt_multiply_binomials
   let _:Prims.unit = assert (Spec.Utils.is_i32b (3328 * 3328 + 3328 * 3328) ai_bj_aj_bi) in
   let _:Prims.unit = assert_norm (3328 * 3328 + 3328 * 3328 <= 3328 * pow2 15) in
   let o1:i16 = Libcrux_ml_kem.Vector.Portable.Arithmetic.montgomery_reduce_element ai_bj_aj_bi in
+  let _:Prims.unit =
+    calc ( == ) {
+      v o1 % 3329;
+      ( == ) { () }
+      (v ai_bj_aj_bi * 169) % 3329;
+      ( == ) { assert (v ai_bj_aj_bi == v ai_bj + v aj_bi) }
+      ((v ai_bj + v aj_bi) * 169) % 3329;
+      ( == ) { assert (v ai_bj == v ai * v bj) }
+      ((v ai * v bj + v aj_bi) * 169) % 3329;
+      ( == ) { assert (v aj_bi == v aj * v bi) }
+      ((v ai * v bj + v aj * v bi) * 169) % 3329;
+    }
+  in
+  let v__out0:t_Array i16 (sz 16) = out.Libcrux_ml_kem.Vector.Portable.Vector_type.f_elements in
   let out:Libcrux_ml_kem.Vector.Portable.Vector_type.t_PortableVector =
     {
       out with
@@ -248,7 +270,7 @@ let ntt_multiply_binomials
       =
       Rust_primitives.Hax.Monomorphized_update_at.update_at_usize out
           .Libcrux_ml_kem.Vector.Portable.Vector_type.f_elements
-        i
+        (sz 2 *! i <: usize)
         o0
     }
     <:
@@ -261,11 +283,18 @@ let ntt_multiply_binomials
       =
       Rust_primitives.Hax.Monomorphized_update_at.update_at_usize out
           .Libcrux_ml_kem.Vector.Portable.Vector_type.f_elements
-        j
+        ((sz 2 *! i <: usize) +! sz 1 <: usize)
         o1
     }
     <:
     Libcrux_ml_kem.Vector.Portable.Vector_type.t_PortableVector
+  in
+  let _:Prims.unit =
+    assert (Seq.index out.f_elements (2 * v i) == o0);
+    assert (Seq.index out.f_elements (2 * v i + 1) == o1);
+    assert (Spec.Utils.is_i16b_array 3328 out.f_elements);
+    assert (forall k.
+          (k <> 2 * v i /\ k <> 2 * v i + 1) ==> Seq.index out.f_elements k == Seq.index v__out0 k)
   in
   let _:Prims.unit = admit () in
   out
@@ -432,30 +461,35 @@ let ntt_multiply
   let out:Libcrux_ml_kem.Vector.Portable.Vector_type.t_PortableVector =
     Libcrux_ml_kem.Vector.Portable.Vector_type.zero ()
   in
+  let _:Prims.unit = assert (Spec.Utils.is_i16b_array 3328 out.f_elements) in
   let out:Libcrux_ml_kem.Vector.Portable.Vector_type.t_PortableVector =
-    ntt_multiply_binomials lhs rhs zeta0 (sz 0) (sz 1) out
+    ntt_multiply_binomials lhs rhs zeta0 (sz 0) out
   in
+  let _:Prims.unit = assert (Spec.Utils.is_i16b_array 3328 out.f_elements) in
   let out:Libcrux_ml_kem.Vector.Portable.Vector_type.t_PortableVector =
-    ntt_multiply_binomials lhs rhs nzeta0 (sz 2) (sz 3) out
+    ntt_multiply_binomials lhs rhs nzeta0 (sz 1) out
   in
+  let _:Prims.unit = assert (Spec.Utils.is_i16b_array 3328 out.f_elements) in
   let out:Libcrux_ml_kem.Vector.Portable.Vector_type.t_PortableVector =
-    ntt_multiply_binomials lhs rhs zeta1 (sz 4) (sz 5) out
+    ntt_multiply_binomials lhs rhs zeta1 (sz 2) out
   in
+  let _:Prims.unit = assert (Spec.Utils.is_i16b_array 3328 out.f_elements) in
   let out:Libcrux_ml_kem.Vector.Portable.Vector_type.t_PortableVector =
-    ntt_multiply_binomials lhs rhs nzeta1 (sz 6) (sz 7) out
+    ntt_multiply_binomials lhs rhs nzeta1 (sz 3) out
   in
+  let _:Prims.unit = assert (Spec.Utils.is_i16b_array 3328 out.f_elements) in
   let _:Prims.unit = admit () in
   let out:Libcrux_ml_kem.Vector.Portable.Vector_type.t_PortableVector =
-    ntt_multiply_binomials lhs rhs zeta2 (sz 8) (sz 9) out
+    ntt_multiply_binomials lhs rhs zeta2 (sz 4) out
   in
   let out:Libcrux_ml_kem.Vector.Portable.Vector_type.t_PortableVector =
-    ntt_multiply_binomials lhs rhs nzeta2 (sz 10) (sz 11) out
+    ntt_multiply_binomials lhs rhs nzeta2 (sz 5) out
   in
   let out:Libcrux_ml_kem.Vector.Portable.Vector_type.t_PortableVector =
-    ntt_multiply_binomials lhs rhs zeta3 (sz 12) (sz 13) out
+    ntt_multiply_binomials lhs rhs zeta3 (sz 6) out
   in
   let out:Libcrux_ml_kem.Vector.Portable.Vector_type.t_PortableVector =
-    ntt_multiply_binomials lhs rhs nzeta3 (sz 14) (sz 15) out
+    ntt_multiply_binomials lhs rhs nzeta3 (sz 7) out
   in
   out
 
