libcrux-ml-kem/proofs/fstar/extraction/Libcrux_ml_kem.Vector.Portable.fst
@@ -1,5 +1,5 @@
 module Libcrux_ml_kem.Vector.Portable
-#set-options "--fuel 0 --ifuel 1 --z3rlimit 15"
+#set-options "--fuel 0 --ifuel 1 --z3rlimit 100"
 open Core
 open FStar.Mul
 
@@ -10,6 +10,50 @@ let _ =
   let open Libcrux_ml_kem.Vector.Traits in
   ()
 
-#push-options "--z3rlimit 300"
+let deserialize_11_ (a: t_Slice u8) = Libcrux_ml_kem.Vector.Portable.Serialize.deserialize_11_ a
 
-#pop-options
+let deserialize_5_ (a: t_Slice u8) = Libcrux_ml_kem.Vector.Portable.Serialize.deserialize_5_ a
+
+let serialize_11_ (a: Libcrux_ml_kem.Vector.Portable.Vector_type.t_PortableVector) =
+  Libcrux_ml_kem.Vector.Portable.Serialize.serialize_11_ a
+
+let serialize_5_ (a: Libcrux_ml_kem.Vector.Portable.Vector_type.t_PortableVector) =
+  Libcrux_ml_kem.Vector.Portable.Serialize.serialize_5_ a
+
+let deserialize_1_ (a: t_Slice u8) =
+  let _:Prims.unit = Libcrux_ml_kem.Vector.Portable.Serialize.deserialize_1_lemma a in
+  let _:Prims.unit = Libcrux_ml_kem.Vector.Portable.Serialize.deserialize_1_bounded_lemma a in
+  Libcrux_ml_kem.Vector.Portable.Serialize.deserialize_1_ a
+
+let deserialize_10_ (a: t_Slice u8) =
+  let _:Prims.unit = Libcrux_ml_kem.Vector.Portable.Serialize.deserialize_10_lemma a in
+  let _:Prims.unit = Libcrux_ml_kem.Vector.Portable.Serialize.deserialize_10_bounded_lemma a in
+  Libcrux_ml_kem.Vector.Portable.Serialize.deserialize_10_ a
+
+let deserialize_12_ (a: t_Slice u8) =
+  let _:Prims.unit = Libcrux_ml_kem.Vector.Portable.Serialize.deserialize_12_lemma a in
+  let _:Prims.unit = Libcrux_ml_kem.Vector.Portable.Serialize.deserialize_12_bounded_lemma a in
+  Libcrux_ml_kem.Vector.Portable.Serialize.deserialize_12_ a
+
+let deserialize_4_ (a: t_Slice u8) =
+  let _:Prims.unit = Libcrux_ml_kem.Vector.Portable.Serialize.deserialize_4_lemma a in
+  let _:Prims.unit = Libcrux_ml_kem.Vector.Portable.Serialize.deserialize_4_bounded_lemma a in
+  Libcrux_ml_kem.Vector.Portable.Serialize.deserialize_4_ a
+
+let serialize_1_ (a: Libcrux_ml_kem.Vector.Portable.Vector_type.t_PortableVector) =
+  let _:Prims.unit = assert (forall i. Rust_primitives.bounded (Seq.index a.f_elements i) 1) in
+  let _:Prims.unit = Libcrux_ml_kem.Vector.Portable.Serialize.serialize_1_lemma a in
+  Libcrux_ml_kem.Vector.Portable.Serialize.serialize_1_ a
+
+let serialize_10_ (a: Libcrux_ml_kem.Vector.Portable.Vector_type.t_PortableVector) =
+  let _:Prims.unit = Libcrux_ml_kem.Vector.Portable.Serialize.serialize_10_lemma a in
+  Libcrux_ml_kem.Vector.Portable.Serialize.serialize_10_ a
+
+let serialize_12_ (a: Libcrux_ml_kem.Vector.Portable.Vector_type.t_PortableVector) =
+  let _:Prims.unit = Libcrux_ml_kem.Vector.Portable.Serialize.serialize_12_lemma a in
+  Libcrux_ml_kem.Vector.Portable.Serialize.serialize_12_ a
+
+let serialize_4_ (a: Libcrux_ml_kem.Vector.Portable.Vector_type.t_PortableVector) =
+  let _:Prims.unit = assert (forall i. Rust_primitives.bounded (Seq.index a.f_elements i) 4) in
+  let _:Prims.unit = Libcrux_ml_kem.Vector.Portable.Serialize.serialize_4_lemma a in
+  Libcrux_ml_kem.Vector.Portable.Serialize.serialize_4_ a
